lib/Lib.Endianness.fsti
@@ -53,3 +53,53 @@ val uint_to_bytes_be:
     (ensures  fun h0 _ h1 ->
       B.live h1 o /\ modifies (loc_buffer o) h0 h1 /\
       B.as_seq h1 o == ByteSeq.uint_to_bytes_be #t i)
+
+inline_for_extraction
+val uints_from_bytes_le:
+  #t:m_inttype -> #len:size_nat{len `op_Multiply` numbytes t <= max_size_t} ->
+  o:lbuffer (uint_t t) (len) ->
+  clen:size_t{size_v clen == len} ->
+  i:lbuffer uint8 (len `op_Multiply` (numbytes t)) ->
+  Stack unit
+	(requires (fun h0 -> B.live h0 o /\ B.live h0 i))
+	(ensures (fun h0 _ h1 -> B.modifies (B.loc_buffer o) h0 h1
+                    /\ B.as_seq h1 o == (ByteSeq.uints_from_bytes_le #t #(len) (B.as_seq h0 i) )))
+
+inline_for_extraction
+val uints_from_bytes_be:
+  #t:m_inttype -> #len:size_nat{len `op_Multiply` numbytes t <= max_size_t} ->
+  o:lbuffer (uint_t t) len ->
+  clen:size_t{size_v clen == len} ->
+  i:lbuffer uint8 (len `op_Multiply` ((numbytes t))) ->
+  Stack unit
+	(requires (fun h0 -> live h0 o /\ live h0 i))
+	(ensures (fun h0 _ h1 -> B.modifies (B.loc_buffer o) h0 h1 /\
+			      B.as_seq h1 o == (ByteSeq.uints_from_bytes_be #t #len (as_seq h0 i) )))
+
+
+inline_for_extraction
+val uints_to_bytes_le:
+  #t:m_inttype -> #len:size_nat{len `op_Multiply` numbytes t <= max_size_t} ->
+  o:lbuffer uint8 (len `op_Multiply` ((numbytes t))) ->
+  clen:size_t{size_v clen == len} ->
+  i:lbuffer (uint_t t) (len) ->
+  Stack unit
+	(requires (fun h0 -> B.live h0 o /\ B.live h0 i))
+	(ensures (fun h0 _ h1 -> B.modifies (B.loc_buffer o) h0 h1 /\
+			      B.as_seq h1 o == (ByteSeq.uints_to_bytes_le #t #(len) (B.as_seq h0 i) )))
+
+inline_for_extraction
+val uints_to_bytes_be:
+  #t:m_inttype -> #len:size_nat{len `op_Multiply` numbytes t <= max_size_t} ->
+  o:lbuffer uint8 (len `op_Multiply` ((numbytes t))) ->
+  clen:size_t{size_v clen == len} ->
+  i:lbuffer (uint_t t) (len) ->
+  Stack unit
+	(requires (fun h0 -> live h0 o /\ live h0 i /\ disjoint o i))
+	(ensures (fun h0 _ h1 -> B.modifies (B.loc_buffer o) h0 h1 /\
+			      B.as_seq h1 o == (ByteSeq.uints_to_bytes_be #t #(len) (B.as_seq h0 i) )))
+
+inline_for_extraction
+let uint32s_to_bytes_le = uints_to_bytes_le #U32
+inline_for_extraction
+let uint32s_from_bytes_le = uints_from_bytes_le #U32
